top level stated, will trickle down next

src/SourceLang.v
@@ -1268,14 +1268,5 @@ Proof.
   congruence.
 Defined.
 
-Require Semantics.
-(*
-Definition Semantics {ty} (exp : expr [] ty) : Semantics.semantics.
-  refine (Semantics.Semantics_gen _ _ _ _ _ _ _).
-  exact (fun x : unit => (@step [] ty)).
-  admit.
-  admit.
-  exact tt.
-  repeat (econstructor; eauto); admit.
-Admitted.
-*)
+
+
