src/MixSemantics.v
@@ -1,0 +1,149 @@
+Require Import Semantics.
+Require Import compcert.common.Smallstep.
+Require Import compcert.common.Globalenvs.
+Require Import compcert.common.Events.
+
+Require Import StructTact.StructTactics.
+Require Import StructTact.Util.
+
+Require Import EricTact.
+
+
+Definition trace_semantics := semantics.
+Definition notrace_semantics := Semantics.semantics.
+
+Definition trace_forward_simulation := forward_simulation.
+Definition notrace_forward_simulation := Semantics.forward_simulation.
+
+(* We need a simulation from notrace to trace *)
+Record mix_forward_simulation (L1 : notrace_semantics) (L2 : trace_semantics) : Type :=
+  Forward_simulation {
+    fsim_index: Type;
+    fsim_order: fsim_index -> fsim_index -> Prop;
+    fsim_order_wf: well_founded fsim_order;
+    fsim_match_states :> fsim_index -> Semantics.state L1 -> state L2 -> Prop;
+    fsim_match_initial_states:
+      forall s1, Semantics.initial_state L1 s1 ->
+      exists i, exists s2, initial_state L2 s2 /\ fsim_match_states i s1 s2;
+    fsim_match_final_states:
+      forall i s1 s2,
+        fsim_match_states i s1 s2 -> Semantics.final_state L1 s1 ->
+        exists r,
+          final_state L2 s2 r;
+    fsim_simulation:
+      forall s1 s1', Semantics.step L1 (Semantics.globalenv L1) s1 s1' ->
+      forall i s2, fsim_match_states i s1 s2 ->
+      exists i', exists s2',
+         (Plus L2 s2 Events.E0 s2' \/ (Star L2 s2 Events.E0 s2' /\ fsim_order i' i))
+      /\ fsim_match_states i' s1' s2';
+    fsim_public_preserved:
+      forall id, Senv.public_symbol (symbolenv L2) id = Senv.public_symbol (Semantics.symbolenv L1) id
+    }.
+
+
+(* Turn a mixed simulation into a sequence of steps *)
+Section SIMULATION_SEQUENCES.
+
+Variable L1: notrace_semantics.
+Variable L2: trace_semantics.
+Variable S: mix_forward_simulation L1 L2.
+
+Lemma simulation_star:
+  forall s1 s1',
+    @Semantics.star (Semantics.genvtype L1) (Semantics.state L1) (Semantics.step L1) (Semantics.globalenv L1) s1 s1' ->
+  forall i s2, S i s1 s2 ->
+  exists i', exists s2', Star L2 s2 Events.E0 s2' /\ S i' s1' s2'.
+Proof.
+  induction 1; intros.
+  exists i; exists s2; split; auto. apply star_refl.
+  exploit fsim_simulation; eauto. intros [i' [s2' [A B]]].
+  exploit IHstar; eauto. intros [i'' [s2'' [C D]]].
+  exists i''; exists s2''; split; auto. eapply star_trans; eauto.
+  2: instantiate (1 := E0); reflexivity.
+  intuition. apply plus_star; auto.
+Qed.
+
+End SIMULATION_SEQUENCES.
+
+
+Section COMPOSE_SIMULATIONS.
+
+Section COMPOSE_NOTRACE_MIX.
+  
+Variable L1: notrace_semantics.
+Variable L2: notrace_semantics.
+Variable L3: trace_semantics.
+Variable S12: notrace_forward_simulation L1 L2.
+Variable S23: mix_forward_simulation L2 L3.
+
+(*
+Let ff_index : Type := (fsim_index _ _ S23 * fsim_index _ _ S12)%type.
+
+Let ff_order : ff_index -> ff_index -> Prop :=
+  lex_ord (clos_trans _ (fsim_order _ _ S23)) (fsim_order _ _ S12).
+
+Let ff_match_states (i: ff_index) (s1: state L1) (s3: state L3) : Prop :=
+  exists s2, S12 (snd i) s1 s2 /\ S23 (fst i) s2 s3.
+*)
+
+Lemma compose_notrace_mix_forward_simulation: mix_forward_simulation L1 L3.
+Proof.
+Admitted.
+(*
+  apply Forward_simulation with (fsim_order := ff_order) (fsim_match_states := ff_match_states).
+(* well founded *)
+  unfold ff_order. apply wf_lex_ord. apply wf_clos_trans. apply fsim_order_wf. apply fsim_order_wf.
+(* initial states *)
+  intros. exploit (fsim_match_initial_states _ _ S12); eauto. intros [i [s2 [A B]]].
+  exploit (fsim_match_initial_states _ _ S23); eauto. intros [i' [s3 [C D]]].
+  exists (i', i); exists s3; split; auto. exists s2; auto.
+(* final states *)
+  intros. destruct H as [s3 [A B]].
+  eapply (fsim_match_final_states _ _ S23); eauto.
+  eapply (fsim_match_final_states _ _ S12); eauto.
+(* simulation *)
+  intros. destruct H0 as [s3 [A B]]. destruct i as [i2 i1]; simpl in *.
+  exploit (fsim_simulation' _ _ S12); eauto. intros [[i1' [s3' [C D]]] | [i1' [C D]]].
+  (* L2 makes one or several steps. *)
+  exploit simulation_plus; eauto. intros [[i2' [s2' [P Q]]] | [i2' [P Q]]].
+  (* L3 makes one or several steps *)
+  exists (i2', i1'); exists s2'; split. auto. exists s3'; auto.
+  (* L3 makes no step *)
+  exists (i2', i1'); exists s2; split.
+  right; split. apply star_refl. red. left. auto.
+  exists s3'; auto.
+  (* L2 makes no step *)
+  exists (i2, i1'); exists s2; split.
+  right; split. apply star_refl. red. right. auto.
+  exists s3; auto.
+(* symbols *)
+  intros. transitivity (Senv.public_symbol (symbolenv L2) id); apply fsim_public_preserved; auto.
+Qed.
+ *)
+End COMPOSE_NOTRACE_MIX.
+
+Section COMPOSE_MIX_TRACE.
+  
+Variable L1: notrace_semantics.
+Variable L2: trace_semantics.
+Variable L3: trace_semantics.
+Variable S12: mix_forward_simulation L1 L2.
+Variable S23: trace_forward_simulation L2 L3.
+
+(*
+Let ff_index : Type := (fsim_index _ _ S23 * fsim_index _ _ S12)%type.
+
+Let ff_order : ff_index -> ff_index -> Prop :=
+  lex_ord (clos_trans _ (fsim_order _ _ S23)) (fsim_order _ _ S12).
+
+Let ff_match_states (i: ff_index) (s1: state L1) (s3: state L3) : Prop :=
+  exists s2, S12 (snd i) s1 s2 /\ S23 (fst i) s2 s3.
+*)
+
+Lemma compose_mix_trace_forward_simulation: mix_forward_simulation L1 L3.
+Proof.
+Admitted.
+  
+End COMPOSE_MIX_TRACE.
+
+End COMPOSE_SIMULATIONS.
